Cook_Levin/IMP-_To_SAS+/IMP_Minus_To_SAS_Plus.thy
@@ -18,8 +18,8 @@ type_synonym SAS_problem = "(IMP_Minus_Minus_To_SAS_Plus_Plus_State_Translations
   IMP_Minus_Minus_To_SAS_Plus_Plus_State_Translations.domain_element) problem" 
 
 lemma le_two_to_the_bit_length_intro: "x \<le> y \<Longrightarrow> x \<le> 2 ^ (bit_length y)"
-  apply(auto simp: bit_length_def)
-  by (metis leD log_exp2_gt max.strict_coboundedI2 max_def)
+  using log_exp2_gt[of y]
+  by (auto simp: bit_length_def)
 
 text \<open> We give a definition to compute the upper bound on the number of bits needed to represent
        all of the fixed input of some IMP- program, the biggest constant therein and all guessed
@@ -29,55 +29,36 @@ definition max_input_bits:: "IMP_Minus_com \<Rightarrow> (vname \<rightharpoonup
 "max_input_bits c I r = 
   bit_length (max (max (Max (ran I)) r) (IMP_Minus_Max_Constant.max_constant c))" 
 
-lemma bit_at_index_geq_max_input_bits_is_zero: "x < r \<Longrightarrow> max_input_bits c I r \<le> b  
-  \<Longrightarrow> nth_bit x b = Zero" 
-proof-
-  assume "x < r" "max_input_bits c I r \<le> b" 
-  hence "bit_length x \<le> bit_length r" using bit_length_monotonic by simp
-  hence "bit_length x \<le> max_input_bits c I r" apply(auto simp: max_input_bits_def)
-    using bit_length_monotonic  by (metis dual_order.trans max.cobounded2 max_def)
-  thus ?thesis using \<open>max_input_bits c I r \<le> b\<close>
-    by(auto simp: max_input_bits_def intro!: bit_geq_bit_length_is_Zero)
-qed
+lemma bit_at_index_geq_max_input_bits_is_zero:
+  assumes "x < r" "max_input_bits c I r \<le> b"
+  shows "nth_bit x b = Zero" 
+  using \<open>x < r\<close>
+  by (fastforce intro: bit_geq_bit_length_is_Zero bit_length_monotonic 
+                       le_trans[OF _ \<open>max_input_bits c I r \<le> b\<close>]
+                simp: max_input_bits_def)
 
-lemma bit_at_index_geq_max_input_bits_is_zero_in_initial_state: "finite (ran I) 
-  \<Longrightarrow> max_input_bits c I r \<le> b
-  \<Longrightarrow> I x = Some y \<Longrightarrow> nth_bit y b = Zero"
-proof-
-  assume "finite (ran I)" "I x = Some y" "max_input_bits c I r \<le> b" 
-  hence "bit_length y \<le> bit_length (Max (ran I))" using bit_length_monotonic
-    by (meson Max_ge ranI)
-  hence "bit_length y \<le> max_input_bits c I r" apply(auto simp: max_input_bits_def)
-    using bit_length_monotonic  by (metis dual_order.trans max.cobounded2 max_def)
-  thus ?thesis using \<open>max_input_bits c I r \<le> b\<close>
-    by(auto simp: max_input_bits_def intro!: bit_geq_bit_length_is_Zero)
-qed
+lemma bit_at_index_geq_max_input_bits_is_zero_in_initial_state:
+  assumes "finite (ran I)" "max_input_bits c I r \<le> b" "I x = Some y" 
+  shows "nth_bit y b = Zero"
+  using assms(1,3)
+  by(fastforce intro: bit_geq_bit_length_is_Zero le_trans[OF _ \<open>max_input_bits c I r \<le> b\<close>] 
+                      Max_ge ranI max.coboundedI1 bit_length_monotonic
+               simp: max_input_bits_def)
 
-lemma max_constant_less_two_to_the_max_input_bits: "max_constant c < 2 ^ (max_input_bits c I r)" 
-  apply(auto simp: max_input_bits_def bit_length_def algebra_simps)
-  using log_exp2_gt max_less_iff_conj by blast
+lemma max_constant_less_two_to_the_max_input_bits:
+  "max_constant c < 2 ^ (max_input_bits c I r)"
+  using log_exp2_gt max_less_iff_conj
+  by(fastforce simp: max_input_bits_def bit_length_def)
 
 lemma initial_state_element_less_two_to_the_max_input_bits: 
-  assumes "finite (ran I)" "I x = Some y" 
-  shows "y < (2 :: nat) ^ (max_input_bits c I r)" 
-proof -
-  have "y \<le> Max (ran I)" using assms by (meson Max_ge ranI)
-  thus ?thesis using log_exp2_gt max_less_iff_conj
-    by(fastforce simp: max_input_bits_def bit_length_def algebra_simps)
-qed
+  "\<lbrakk>finite (ran I); I x = Some y\<rbrakk> \<Longrightarrow> y < (2 :: nat) ^ (max_input_bits c I r)" 
+  by(force intro: log_exp2_gt Max_ge ranI order.strict_trans1[of y "Max (ran I)"]
+                  order.strict_trans1[of _ "(max (max (Max (ran I)) r) (max_constant c))"]
+           simp: algebra_simps max_input_bits_def bit_length_def)
 
 text \<open> Translation of a (partial) initial state from IMP- to IMP--. Observe that in order to avoid
-       overflows when executing IMP--, we require all bits in in the bit blasted IMP-- registers
-       that are unspecified in the IMP- initial state to be zero. \<close>
-
-definition IMP_Minus_initial_to_IMP_Minus_Minus:: "(vname \<rightharpoonup> nat) 
-  \<Rightarrow> nat \<Rightarrow> nat \<Rightarrow> (vname \<rightharpoonup> bit)" where
-"IMP_Minus_initial_to_IMP_Minus_Minus I n guess_range = (\<lambda>v. 
-  (case var_to_operand_bit v of 
-    Some (CHR ''a'', k) \<Rightarrow> if k < n then Some Zero else None |
-    Some (CHR ''b'', k) \<Rightarrow> if k < n then Some Zero else None | 
-    _ \<Rightarrow> (if v = ''carry'' then Some Zero 
-  else (IMP_Minus_State_To_IMP_Minus_Minus_partial I n guess_range) v)))" 
+       overflows when executing IMP--, we require all bits beyond a certain guess_range in the bit
+       blasted IMP-- registers that are unspecified in the IMP- initial state to be zero. \<close>
 
 text \<open> We give our reduction, by composing the steps IMP- \<Rightarrow> IMP-- \<Rightarrow> SAS++ \<Rightarrow> SAS+. For the IMP-
        \<Rightarrow> IMP-- step, we compute a number of bits n that is guaranteed to suffice for all
@@ -87,16 +68,19 @@ text \<open> We give our reduction, by composing the steps IMP- \<Rightarrow> IM
 
 definition IMP_Minus_to_SAS_Plus:: "IMP_Minus_com \<Rightarrow> (vname \<rightharpoonup> nat) \<Rightarrow> nat \<Rightarrow> (vname \<rightharpoonup> nat) 
   \<Rightarrow>  nat \<Rightarrow> SAS_problem" where
-"IMP_Minus_to_SAS_Plus c I r G t = (let 
-  guess_range = max_input_bits c I r;
-  n = t + guess_range + 1;
-  c' = IMP_Minus_To_IMP_Minus_Minus c n;
-  I' = IMP_Minus_initial_to_IMP_Minus_Minus I n guess_range
-    |` (set (enumerate_variables c')) ;
-  G' = (IMP_Minus_State_To_IMP_Minus_Minus_partial G n n) |` (set (enumerate_variables c')) in 
-  SAS_Plus_Plus_To_SAS_Plus (imp_minus_minus_to_sas_plus c' I' G'))"
+"IMP_Minus_to_SAS_Plus c I r G t =
+ (let 
+    guess_range = max_input_bits c I r;
+    n = t + guess_range + 1;
+    c' = IMP_Minus_To_IMP_Minus_Minus c n;
+    I' = IMP_Minus_State_To_IMP_Minus_Minus_partial I n guess_range |` (set (enumerate_variables c'));
+    G' = (IMP_Minus_State_To_IMP_Minus_Minus_partial G n n) |` (set (enumerate_variables c'));
+    sas_pp = imp_minus_minus_to_sas_plus c' I' G';
+    sas_p = SAS_Plus_Plus_To_SAS_Plus sas_pp
+  in 
+    sas_p)"
 
-lemma le_mul_intro: "0 < b \<Longrightarrow> a \<le> b \<Longrightarrow> (1 :: nat) < c \<Longrightarrow> a < c * b" 
+lemma le_mul_intro: "0 < b \<Longrightarrow> a \<le> b \<Longrightarrow> (1 :: nat) < c \<Longrightarrow> a < c * b"
   by (metis One_nat_def dual_order.strict_trans le_neq_implies_less n_less_m_mult_n)
 
 text \<open> First direction of the correctness proof for the IMP- to SAS+ reduction, showing that when
@@ -104,7 +88,34 @@ text \<open> First direction of the correctness proof for the IMP- to SAS+ reduc
       goal state that matches the end state of the IMP- program, such that the plan is polynomially
       longer than the execution in IMP-. The constants used to bound the length of the plan have
       no significance, rather they are just derived by adding up the various constants that we
-      used in the correctness proofs for the different parts of the reduction. \<close> 
+      used in the correctness proofs for the different parts of the reduction. \<close>           
+
+lemma map_le_proj: "m1 \<subseteq>\<^sub>m m2 \<Longrightarrow> m1 |` s \<subseteq>\<^sub>m m2 |` s"
+  by (auto simp: map_le_def)
+
+lemma map_le_IMP_Minus_State_To_IMP_Minus_Minus:
+  "\<lbrakk>s1 \<subseteq>\<^sub>m Some \<circ> s2\<rbrakk> \<Longrightarrow>
+   IMP_Minus_State_To_IMP_Minus_Minus_partial s1 n n \<subseteq>\<^sub>m IMP_Minus_State_To_IMP_Minus_Minus s2 n"
+    apply (auto simp: IMP_Minus_State_To_IMP_Minus_Minus_partial_def
+                   IMP_Minus_State_To_IMP_Minus_Minus_def
+                   IMP_Minus_State_To_IMP_Minus_Minus_with_operands_a_b_def
+                   map_le_def
+             split!: option.splits if_splits char.splits bool.splits)
+    by (smt domI map_comp_Some_iff option.inject)+
+
+lemma map_le_IMP_Minus_State_To_IMP_Minus_Minus_2:
+  "\<lbrakk>s1 \<subseteq>\<^sub>m Some \<circ> s2; range s2 \<noteq> {}; finite (range s2); Max (range s2) < r; (bit_length r) \<le> rbl\<rbrakk> \<Longrightarrow>
+   IMP_Minus_State_To_IMP_Minus_Minus_partial s1 n rbl \<subseteq>\<^sub>m IMP_Minus_State_To_IMP_Minus_Minus s2 n"
+    apply (auto simp: IMP_Minus_State_To_IMP_Minus_Minus_partial_def
+                   IMP_Minus_State_To_IMP_Minus_Minus_def
+                   IMP_Minus_State_To_IMP_Minus_Minus_with_operands_a_b_def
+                   map_le_def image_def
+             split!: option.splits if_splits char.splits bool.splits)
+   apply (smt domI map_comp_Some_iff option.inject)
+  apply(intro bit_geq_bit_length_is_Zero[symmetric])
+  by (metis bit_length_monotonic leI le_less less_le_trans)
+
+
 
 lemma IMP_Minus_to_SAS_Plus_correctness:
   assumes
@@ -113,99 +124,114 @@ lemma IMP_Minus_to_SAS_Plus_correctness:
     "Max (range s1) < r"
     "G \<subseteq>\<^sub>m Some \<circ> s2"
     "(c, s1) \<Rightarrow>\<^bsup>t\<^esup> s2"
-  shows "\<exists>plan. length plan \<le> 100 * (max_input_bits c I r + t + 1) * (t - 1) 
-      + (max_input_bits c I r + t + 1 + 1) * (num_variables c + 2) + 52
-      \<and> is_serial_solution_for_problem (IMP_Minus_to_SAS_Plus c I r G t) plan"
+    "t \<le> t'"
+  shows
+    "\<exists>plan. length plan \<le> 100 * (max_input_bits c I r + t' + 1) * (t' - 1) 
+                            + (max_input_bits c I r + t' + 1 + 1) * (num_variables c + 2) + 52
+            \<and> is_serial_solution_for_problem (IMP_Minus_to_SAS_Plus c I r G t') plan"
 proof -
   let ?guess_range = " max_input_bits c I r"
-  let ?n = "t + ?guess_range + 1"
+  let ?n = "?guess_range + t' + 1"
   let ?c' = "IMP_Minus_To_IMP_Minus_Minus c ?n"
   let ?s1' = "IMP_Minus_State_To_IMP_Minus_Minus s1 ?n |` (set (enumerate_variables ?c'))"
   let ?s2' = "IMP_Minus_State_To_IMP_Minus_Minus s2 ?n |` (set (enumerate_variables ?c'))"
-  let ?I = "(IMP_Minus_initial_to_IMP_Minus_Minus I ?n ?guess_range) 
+  let ?I = "(IMP_Minus_State_To_IMP_Minus_Minus_partial I ?n ?guess_range) 
     |` (set (enumerate_variables ?c'))"
   let ?G = "(IMP_Minus_State_To_IMP_Minus_Minus_partial G ?n ?n) 
     |` (set (enumerate_variables ?c'))"
-  let ?t = "100 * ?n * (t - 1) + 51"
+  let ?t = "100 * ?n * (t' - 1) + 51"
   let ?sas_plus_plus_problem 
-    = "imp_minus_minus_to_sas_plus (IMP_Minus_To_IMP_Minus_Minus c ?n) ?I ?G"
+    = "imp_minus_minus_to_sas_plus ?c' ?I ?G"
 
   have "?n > 0" by simp
 
-  have "t_small_step_fun (100 * ?n * (t - 1) + 50) 
+  have "Suc 0 < 2 ^ t'"
+    using \<open>(c, s1) \<Rightarrow>\<^bsup> t \<^esup> s2\<close> \<open>t \<le> t'\<close> log_Suc_zero
+    by (fastforce intro: Suc_lessI dest: bigstep_progress)
+  moreover have "2 ^ t * max (Max (range s1)) (max_constant c) \<le> 2 ^ t' * 2 ^ max_input_bits c I r"
+           (is "?max_bits_t \<le> _")
+    using \<open>Max (range s1) < r\<close> \<open>t \<le> t'\<close> le_two_to_the_bit_length_intro mult_le_mono
+    by (auto simp: max_input_bits_def)
+  ultimately have "?max_bits_t < 2 ^ (t' + max_input_bits c I r + 1)"
+    by(auto simp: power_add intro!: le_mul_intro)
+  moreover have "t < t' + max_input_bits c I r + 1"
+    using assms
+    by auto
+
+  ultimately have "t_small_step_fun (100 * ?n * (t - 1) + 50)
       (IMP_Minus_To_IMP_Minus_Minus c ?n, IMP_Minus_State_To_IMP_Minus_Minus s1 ?n)
      = (SKIP, IMP_Minus_State_To_IMP_Minus_Minus s2 ?n)" 
-    apply - apply(rule IMP_Minus_To_IMP_Minus_Minus)
-    using assms apply(auto simp: max.strict_coboundedI1 max.strict_coboundedI2 max_input_bits_def 
-        power_add intro!: le_mul_intro le_two_to_the_bit_length_intro) 
-    by (metis less_imp_le_nat max.coboundedI1 max.commute)
-
-  then have "\<exists>t' \<le> 100 * ?n * (t - 1) + 50. (?c', ?s1') \<rightarrow>\<^bsup>t'\<^esup> (SKIP, ?s2')" 
-    apply -  apply(rule iffD1[OF t_small_step_fun_t_small_step_equivalence])
-    by(auto simp: t_small_step_fun_restrict_variables)
-  then obtain t' where t'_def: "t' \<le> 100 * ?n * (t - 1) + 50" "(?c', ?s1') \<rightarrow>\<^bsup>t'\<^esup> (SKIP, ?s2')" 
+    using assms(2,5)
+    by (fastforce intro!: IMP_Minus_To_IMP_Minus_Minus simp: add.commute)+
+  moreover have "(100 * ?n * (t - 1) + 50) \<le> (100 * ?n * (t' - 1) + 50)"
+    using \<open>t \<le> t'\<close>
+    by auto
+  ultimately have 
+    "t_small_step_fun (100 * ?n * (t' - 1) + 50) (?c', IMP_Minus_State_To_IMP_Minus_Minus s1 ?n)
+       = (SKIP, IMP_Minus_State_To_IMP_Minus_Minus s2 ?n)" 
+    using t_small_step_fun_increase_time by blast
+  hence "\<exists>t'' \<le> 100 * ?n * (t' - 1) + 50. (?c', ?s1') \<rightarrow>\<^bsup>t''\<^esup> (SKIP, ?s2')" 
+    by(auto simp: t_small_step_fun_restrict_variables
+            intro: iffD1[OF t_small_step_fun_t_small_step_equivalence])
+  then obtain t'' where t''_def: "t'' \<le> 100 * ?n * (t' - 1) + 50" "(?c', ?s1') \<rightarrow>\<^bsup>t''\<^esup> (SKIP, ?s2')" 
     by blast
 
-  hence "?G v = Some y \<Longrightarrow> ?s2' v = Some y" for v y
-    using \<open>G \<subseteq>\<^sub>m Some \<circ> s2\<close> 
-    apply(auto simp: IMP_Minus_State_To_IMP_Minus_Minus_def var_to_var_bit_eq_Some_iff
-          IMP_Minus_State_To_IMP_Minus_Minus_with_operands_a_b_def 
-           IMP_Minus_State_To_IMP_Minus_Minus_partial_def map_le_def map_comp_def dom_def
-           split!: option.splits if_splits char.splits bool.splits)
-    apply(frule var_bit_in_IMP_Minus_Minus_variables_then_bit_less_n[OF \<open>?n > 0\<close>, simplified])
-    by simp
-  hence "?G \<subseteq>\<^sub>m ?s2'" by (auto simp: map_le_def)
+  have "?G \<subseteq>\<^sub>m ?s2'"
+    by (intro map_le_proj map_le_IMP_Minus_State_To_IMP_Minus_Minus[OF \<open>G \<subseteq>\<^sub>m Some \<circ> s2\<close>])
 
-  have "?I v = Some y \<Longrightarrow> ?s1' v = Some y" for v y
-    apply auto
-    apply(drule set_mp[OF IMP_Minus_To_IMP_Minus_Minus_variables[OF \<open>?n > 0\<close>, simplified]])
-    apply(cases "v = ''carry''")
-    using \<open>I \<subseteq>\<^sub>m Some \<circ> s1\<close>
-     apply(auto simp: IMP_Minus_State_To_IMP_Minus_Minus_partial_def 
-        IMP_Minus_State_To_IMP_Minus_Minus_with_operands_a_b_def dom_def
-        IMP_Minus_State_To_IMP_Minus_Minus_def map_comp_def map_le_def 
-        IMP_Minus_initial_to_IMP_Minus_Minus_def
-        split: if_splits option.splits)
-    using \<open>finite (range s1)\<close> \<open>Max (range s1) < r\<close> 
-    by(auto intro: bit_at_index_geq_max_input_bits_is_zero)
-  hence "?I  \<subseteq>\<^sub>m ?s1'" by (auto simp: map_le_def)
+  have "?I  \<subseteq>\<^sub>m ?s1'"
+    by (auto simp: range max_input_bits_def
+             intro!: map_le_proj bit_length_monotonic
+                     map_le_IMP_Minus_State_To_IMP_Minus_Minus_2
+                      [OF \<open>I \<subseteq>\<^sub>m Some \<circ> s1\<close> _ \<open>finite (range s1)\<close> \<open>Max (range s1) < r\<close>])
 
   let ?ss1'' = "imp_minus_state_to_sas_plus (?c', ?s1')" 
-  let ?ss2'' = "imp_minus_state_to_sas_plus (SKIP, ?s2')" 
-  obtain plan where plan_def: 
+  let ?ss2'' = "imp_minus_state_to_sas_plus (SKIP, ?s2')"
+                                                          
+  thm set_mp[OF IMP_Minus_To_IMP_Minus_Minus_variables[OF \<open>?n > 0\<close>, simplified]]
+                                                                    
+  obtain plan where plan_def:
      "is_serial_solution_for_problem_sas_plus_plus ?sas_plus_plus_problem plan"
-     "length plan = t'"
-    apply- apply(rule exE[OF imp_minus_minus_to_sas_plus_plus[OF \<open>(?c', ?s1') \<rightarrow>\<^bsup>t'\<^esup> (SKIP, ?s2')\<close>,
-            where ?I="?I" and ?G="?G"]])
-       apply auto
-      apply(drule set_mp[OF IMP_Minus_To_IMP_Minus_Minus_variables[OF \<open>?n > 0\<close>, simplified]])
-      using \<open>?I  \<subseteq>\<^sub>m ?s1'\<close> \<open>?G \<subseteq>\<^sub>m ?s2'\<close> by(auto simp: IMP_Minus_State_To_IMP_Minus_Minus_def 
-        IMP_Minus_State_To_IMP_Minus_Minus_with_operands_a_b_def)
+     "length plan \<le> t''"
+    apply(rule exE[OF imp_minus_minus_to_sas_plus_plus[OF \<open>(?c', ?s1') \<rightarrow>\<^bsup>t''\<^esup> (SKIP, ?s2')\<close>,
+                      where ?I="?I" and ?G="?G" and t' = t'']])
+    using \<open>?I  \<subseteq>\<^sub>m ?s1'\<close> \<open>?G \<subseteq>\<^sub>m ?s2'\<close> 
+    by (auto simp add: dom_of_IMP_Minus_State_To_IMP_Minus_Minus 
+        dest: set_mp[OF IMP_Minus_To_IMP_Minus_Minus_variables[OF \<open>?n > 0\<close>, simplified]])
 
-   hence "\<exists>prefix. length prefix \<le> length ((?sas_plus_plus_problem)\<^sub>\<V>\<^sub>+) + 1 
-    \<and> is_serial_solution_for_problem (SAS_Plus_Plus_To_SAS_Plus ?sas_plus_plus_problem) 
-        (prefix @ (map SAS_Plus_Plus_Operator_To_SAS_Plus_Operator plan))"
-     apply -
-     apply(rule SAS_Plus_Plus_To_SAS_Plus)
-     apply(rule imp_minus_minus_to_sas_plus_valid)
-     by(auto simp: IMP_Minus_State_To_IMP_Minus_Minus_partial_def map_comp_def 
-         split: option.splits)
-   then obtain prefix where prefix_def: "length prefix \<le> length ((?sas_plus_plus_problem)\<^sub>\<V>\<^sub>+) + 1 
-    \<and> is_serial_solution_for_problem (SAS_Plus_Plus_To_SAS_Plus ?sas_plus_plus_problem) 
-        (prefix @ (map SAS_Plus_Plus_Operator_To_SAS_Plus_Operator plan))" by blast
+   hence "\<exists>prefix. length prefix \<le> length ((?sas_plus_plus_problem)\<^sub>\<V>\<^sub>+) + 1
+                   \<and> is_serial_solution_for_problem
+                        (SAS_Plus_Plus_To_SAS_Plus ?sas_plus_plus_problem) 
+                        (prefix @ (map SAS_Plus_Plus_Operator_To_SAS_Plus_Operator plan))"
+     by(fastforce simp: IMP_Minus_State_To_IMP_Minus_Minus_partial_def map_comp_def 
+                  intro!: SAS_Plus_Plus_To_SAS_Plus imp_minus_minus_to_sas_plus_valid
+                  split: option.splits)
+
+   then obtain prefix where
+     prefix_def: "length prefix \<le> length ((?sas_plus_plus_problem)\<^sub>\<V>\<^sub>+) + 1
+                  \<and> is_serial_solution_for_problem 
+                       (SAS_Plus_Plus_To_SAS_Plus ?sas_plus_plus_problem) 
+                       (prefix @ (map SAS_Plus_Plus_Operator_To_SAS_Plus_Operator plan))"
+     by rule
+
    let ?plan' = "prefix @ (map SAS_Plus_Plus_Operator_To_SAS_Plus_Operator plan)"
-   have "length ((?sas_plus_plus_problem)\<^sub>\<V>\<^sub>+) \<le> (?n + 1) * (num_variables c + 2) + 1" using 
-     IMP_Minus_To_IMP_Minus_Minus_variables_length[where ?c=c 
-         and ?n="(Suc (t + max_input_bits c I r))"] 
-     by(auto simp: imp_minus_minus_to_sas_plus_def Let_def)
-   hence "length prefix \<le> (?n + 1) * (num_variables c + 2) + 2" using prefix_def by simp
-   hence "length ?plan' \<le> 100 * ?n * (t - 1) + (?n + 1) * (num_variables c + 2) + 52
-      \<and> is_serial_solution_for_problem (IMP_Minus_to_SAS_Plus c I r G t) ?plan'"
-     using plan_def prefix_def t'_def by(auto simp: IMP_Minus_to_SAS_Plus_def Let_def)
-   thus ?thesis by (metis add.commute)
+   have "length ((?sas_plus_plus_problem)\<^sub>\<V>\<^sub>+) \<le> (?n + 1) * (num_variables c + 2) + 1"
+     using IMP_Minus_To_IMP_Minus_Minus_variables_length
+             [where ?c=c and ?n="(Suc (t' + max_input_bits c I r))"]
+     by(auto simp: imp_minus_minus_to_sas_plus_def Let_def add.commute)
+   hence "length prefix \<le> (?n + 1) * (num_variables c + 2) + 2"
+     using prefix_def
+     by simp
+   hence "length ?plan' \<le> 100 * ?n * (t' - 1) + (?n + 1) * (num_variables c + 2) + 52
+           \<and> is_serial_solution_for_problem (IMP_Minus_to_SAS_Plus c I r G t') ?plan'"
+     using plan_def prefix_def t''_def
+     by(auto simp: IMP_Minus_to_SAS_Plus_def Let_def add.commute)
+   thus ?thesis
+     by rule
 qed
 
-lemma not_in_superset_of_dom_then_None: "dom s \<subseteq> S \<Longrightarrow> x \<notin> S \<Longrightarrow> s x = None" by auto
+lemma not_in_superset_of_dom_then_None:
+ "dom s \<subseteq> S \<Longrightarrow> x \<notin> S \<Longrightarrow> s x = None" by auto
 
 text \<open> Second direction of the correctness proof. We show that for an IMP- program that will
       terminate after at most t steps on any input, if there is a solution in the reduced 
@@ -219,13 +245,13 @@ lemma SAS_Plus_to_IMP_Minus_correctness:
     "dom G \<subseteq> set (IMP_Minus_Max_Constant.all_variables c)" 
     "Max (ran G) < 2 ^ (t + max_input_bits c I r)" 
     "is_serial_solution_for_problem (IMP_Minus_to_SAS_Plus c I r G t) plan"
-    "\<forall>s1. \<exists>s2. \<exists>t' \<le> t. (c, s1) \<Rightarrow>\<^bsup>t'\<^esup> s2" 
+    "\<forall>s1. I \<subseteq>\<^sub>m Some o s1 \<longrightarrow> (\<exists>s2. \<exists>t' \<le> t. (c, s1) \<Rightarrow>\<^bsup>t'\<^esup> s2)" 
   shows "\<exists>s1 s2 t'. t' \<le> t \<and> I \<subseteq>\<^sub>m Some \<circ> s1 \<and> G \<subseteq>\<^sub>m Some \<circ> s2 \<and> (c, s1)  \<Rightarrow>\<^bsup>t'\<^esup> s2" 
 proof -
   let ?guess_range = "max_input_bits c I r"
   let ?n = "t + ?guess_range + 1"
   let ?c' = "IMP_Minus_To_IMP_Minus_Minus c ?n"
-  let ?I = "(IMP_Minus_initial_to_IMP_Minus_Minus I ?n ?guess_range) 
+  let ?I = "(IMP_Minus_State_To_IMP_Minus_Minus_partial I ?n ?guess_range) 
     |` (set (enumerate_variables ?c'))"
   let ?G = "(IMP_Minus_State_To_IMP_Minus_Minus_partial G ?n ?n) |` (set (enumerate_variables ?c'))"
 
@@ -263,12 +289,12 @@ proof -
       thus ?thesis using \<open>v \<in> set (enumerate_variables ?c')\<close> 
           apply(auto simp: IMP_Minus_State_To_IMP_Minus_Minus_partial_def  
               IMP_Minus_State_To_IMP_Minus_Minus_with_operands_a_b_def var_to_var_bit_eq_Some_iff
-              var_to_operand_bit_eq_Some_iff IMP_Minus_initial_to_IMP_Minus_Minus_def
+              var_to_operand_bit_eq_Some_iff 
               IMP_Minus_State_To_IMP_Minus_Minus_partial_of_operand_bit_to_var
               IMP_Minus_State_To_IMP_Minus_Minus_def
               nth_bit_of_IMP_Minus_Minus_State_To_IMP_Minus 
               split: option.splits)
-        using \<open>v \<in> dom ?I\<close> by(auto simp: map_comp_def IMP_Minus_initial_to_IMP_Minus_Minus_def 
+        using \<open>v \<in> dom ?I\<close> by(auto simp: map_comp_def 
             IMP_Minus_State_To_IMP_Minus_Minus_partial_def
             IMP_Minus_State_To_IMP_Minus_Minus_partial_of_operand_bit_to_var 
             var_bit_to_var_neq_operand_bit_to_var[symmetric]
@@ -279,7 +305,7 @@ proof -
       then obtain v' i where "v = var_bit_to_var (v', i) \<and> i < ?guess_range" using \<open>\<not>(v \<in> dom ?I)\<close>
          \<open>v \<in> set (enumerate_variables ?c')\<close>
         set_mp[OF IMP_Minus_To_IMP_Minus_Minus_variables \<open>v \<in> set (enumerate_variables ?c')\<close>]
-        apply(auto simp: IMP_Minus_initial_to_IMP_Minus_Minus_def map_comp_def
+        apply(auto simp: map_comp_def
             IMP_Minus_State_To_IMP_Minus_Minus_partial_def split: option.splits)
         using leI by blast
       thus ?thesis using \<open>v \<in> set (enumerate_variables ?c')\<close> 
@@ -294,25 +320,29 @@ proof -
   qed
   hence "s1 = IMP_Minus_State_To_IMP_Minus_Minus ?s1' ?n |` (set (enumerate_variables ?c'))" by auto
 
-  have "I v = Some y \<Longrightarrow> ?s1' v = y" for v y 
+  have "?s1' v = y" if "I v = Some y" for v y 
   proof -
-    assume "I v = Some y" 
-    hence "v \<in> set (IMP_Minus_Max_Constant.all_variables c)" 
-      using \<open>dom I \<subseteq> set (IMP_Minus_Max_Constant.all_variables c)\<close> by auto
+    from that have "v \<in> set (IMP_Minus_Max_Constant.all_variables c)" 
+      using \<open>dom I \<subseteq> set (IMP_Minus_Max_Constant.all_variables c)\<close>
+      by auto
     hence "\<forall>i < ?n. var_bit_to_var (v, i) \<in> set (enumerate_variables ?c')" 
       by(auto simp: var_bit_in_IMP_Minus_Minus_variables)
-    moreover hence "i < ?n \<longrightarrow> s1 (var_bit_to_var (v, i)) = ?I (var_bit_to_var (v, i))" for i
+    moreover hence "i < ?n \<Longrightarrow> s1 (var_bit_to_var (v, i)) = ?I (var_bit_to_var (v, i))" for i
       using \<open>(?I|` set (enumerate_variables ?c')) \<subseteq>\<^sub>m s1\<close> \<open>I v = Some y\<close>
-      by(auto simp: IMP_Minus_initial_to_IMP_Minus_Minus_def map_le_def
-          IMP_Minus_State_To_IMP_Minus_Minus_def dom_def
-          IMP_Minus_State_To_IMP_Minus_Minus_partial_def map_comp_def split: option.splits) 
-    ultimately show "?s1' v = y" using \<open>(?I|` set (enumerate_variables ?c')) \<subseteq>\<^sub>m s1\<close>
-       less_le_trans[OF initial_state_element_less_two_to_the_max_input_bits[where ?c=c and ?r=r]]
-       \<open>I v = Some y\<close> bit_at_index_geq_max_input_bits_is_zero_in_initial_state \<open>finite (ran I)\<close>
-      by(fastforce simp add: IMP_Minus_initial_to_IMP_Minus_Minus_def map_comp_def 
-          IMP_Minus_Minus_State_To_IMP_Minus_def power_add 
+      by(auto simp: map_le_def
+                    IMP_Minus_State_To_IMP_Minus_Minus_def dom_def
+                    IMP_Minus_State_To_IMP_Minus_Minus_partial_def map_comp_def
+              split: option.splits) 
+    ultimately show "?s1' v = y"
+      using
+        \<open>(?I|` set (enumerate_variables ?c')) \<subseteq>\<^sub>m s1\<close>
+        less_le_trans[OF initial_state_element_less_two_to_the_max_input_bits[where ?c=c and ?r=r]]
+        \<open>I v = Some y\<close> bit_at_index_geq_max_input_bits_is_zero_in_initial_state \<open>finite (ran I)\<close>
+      by(auto si mp add: map_comp_def 
+           power_add 
           algebra_simps nth_append bit_list_to_nat_eq_nat_iff
-          IMP_Minus_State_To_IMP_Minus_Minus_partial_def split: if_splits option.splits)
+          IMP_Minus_State_To_IMP_Minus_Minus_partial_def map_le_def
+ split: if_splits option.splits bool.splits char.splits)
   qed
   hence "I \<subseteq>\<^sub>m Some \<circ> ?s1'" by(auto simp: map_le_def)
   
@@ -331,17 +361,18 @@ proof -
     = (SKIP, s2')" "s2' |` set (enumerate_variables ?c') = s2" by auto (metis prod.collapse)
 
   moreover obtain t'' s2'' where "t'' \<le> t" "(c, ?s1') \<Rightarrow>\<^bsup>t''\<^esup> s2''" 
-    using \<open>\<forall>s1. \<exists>s2. \<exists>t' \<le> t. (c, s1) \<Rightarrow>\<^bsup>t'\<^esup> s2\<close> by blast
+    using \<open>\<forall>s1. I \<subseteq>\<^sub>m Some o s1 \<longrightarrow> (\<exists>s2. \<exists>t' \<le> t. (c, s1) \<Rightarrow>\<^bsup>t'\<^esup> s2)\<close>
+    using \<open>I \<subseteq>\<^sub>m Some \<circ> IMP_Minus_Minus_State_To_IMP_Minus s1 (t + max_input_bits c I r + 1)\<close>
+    by blast
   moreover have "?guess_range \<le> i \<Longrightarrow> s1 (var_bit_to_var (v, i)) \<noteq> Some One" for i v 
   proof(cases "(var_bit_to_var (v, i)) \<in> set (enumerate_variables ?c')")
     case True
     assume "?guess_range \<le> i"
     hence "?I (var_bit_to_var (v, i)) = Some Zero" 
       using \<open>(var_bit_to_var (v, i)) \<in> set (enumerate_variables ?c')\<close>  
-      by(auto simp: IMP_Minus_initial_to_IMP_Minus_Minus_def 
-          IMP_Minus_State_To_IMP_Minus_Minus_partial_def 
-          dest!: set_mp[OF IMP_Minus_To_IMP_Minus_Minus_variables]
-          split: option.splits)
+      by(auto simp: IMP_Minus_State_To_IMP_Minus_Minus_partial_def 
+              dest!: set_mp[OF IMP_Minus_To_IMP_Minus_Minus_variables]
+              split: option.splits)
     thus ?thesis using \<open>(?I|` set (enumerate_variables ?c')) \<subseteq>\<^sub>m s1\<close> by(auto simp: map_le_def dom_def)
   next
     case False
@@ -364,7 +395,7 @@ proof -
       by(auto simp: var_bit_in_IMP_Minus_Minus_variables)
     moreover hence "i < ?n \<longrightarrow> s2 (var_bit_to_var (v, i)) = ?G (var_bit_to_var (v, i))" for i
       using \<open>(?G|` set (enumerate_variables ?c')) \<subseteq>\<^sub>m s2\<close> \<open>G v = Some y\<close>
-      by(auto simp: IMP_Minus_initial_to_IMP_Minus_Minus_def map_le_def
+      by(auto simp:  map_le_def
           IMP_Minus_State_To_IMP_Minus_Minus_def dom_def
           IMP_Minus_State_To_IMP_Minus_Minus_partial_def map_comp_def split: option.splits) 
     moreover hence "i < ?n \<longrightarrow> s2' (var_bit_to_var (v, i)) = ?G (var_bit_to_var (v, i))" for i 
